TODO.md
@@ -1,6 +1,5 @@
 ## To-do list
 
-- About `first_unioncharset`: does the outcome depend on the boolean return value?
 - Define a functional version of  `first` and its equivalence to the inductive definition
 - Think the case for the and-predicate patterns `&P` in the definition of first in C: can we make the case for the not-predicate pattern `!P` stronger?
   Is there something that first can return and make the definition more informative?
